Isabelle/LatestMessage.thy
@@ -4,43 +4,50 @@ imports Main CBCCasper
 
 begin
 
+(* ###################################################### *)
 (* Section 4: Example Protocols *)
+(* ###################################################### *)
+
 (* Section 4.1:  Preliminary Definitions *)
 
 (* Definition 4.2 *)
-fun later :: "(message * state) \<Rightarrow> message set"
+definition later :: "(message * state) \<Rightarrow> message set"
   where
-    "later (m, \<sigma>) = {m' \<in> \<sigma>. justified m m'}"
+    "later = (\<lambda>(m, \<sigma>). {m' \<in> \<sigma>. justified m m'})"
 
 lemma (in Protocol) later_type :
   "\<forall> \<sigma> m. \<sigma> \<in> \<Sigma> \<and> m \<in> M \<longrightarrow> later (m, \<sigma>) \<subseteq> M"
+  apply (simp add: later_def)
   using state_is_subset_of_M by auto
 
 (* Definition 4.3: Messages From a Sender *)
-fun  from_sender :: "(validator * state) \<Rightarrow> message set"
+definition from_sender :: "(validator * state) \<Rightarrow> message set"
   where
-    "from_sender (v, \<sigma>) = {m \<in> \<sigma>. sender m = v}"
+    "from_sender  = (\<lambda>(v, \<sigma>). {m \<in> \<sigma>. sender m = v})"
 
 lemma (in Protocol) from_sender_type :
   "\<forall> \<sigma> v. \<sigma> \<in> \<Sigma> \<and> v \<in> V \<longrightarrow> from_sender (v, \<sigma>) \<subseteq> M"
+  apply (simp add: from_sender_def)
   using state_is_subset_of_M by auto  
 
 (* Definition 4.4: Message From a Group *)
-fun from_group :: "(validator set * state) \<Rightarrow> state"
+definition from_group :: "(validator set * state) \<Rightarrow> state"
   where
-    "from_group (v_set, \<sigma>) = {m \<in> \<sigma>. sender m \<in> v_set}"
+    "from_group = (\<lambda>(v_set, \<sigma>). {m \<in> \<sigma>. sender m \<in> v_set})"
 
 lemma (in Protocol) from_group_type :
   "\<forall> \<sigma> v. \<sigma> \<in> \<Sigma> \<and> v_set \<subseteq> V \<longrightarrow> from_group (v_set, \<sigma>) \<subseteq> M"
+  apply (simp add: from_group_def)
   using state_is_subset_of_M by auto
 
 (* Definition 4.5 *)
-fun later_from :: "(message * validator * state) \<Rightarrow> message set"
+definition later_from :: "(message * validator * state) \<Rightarrow> message set"
   where
-    "later_from (m, v, \<sigma>) = later (m, \<sigma>) \<inter> from_sender (v, \<sigma>)"
+    "later_from = (\<lambda>(m, v, \<sigma>). later (m, \<sigma>) \<inter> from_sender (v, \<sigma>))"
 
 lemma (in Protocol) later_from_type :
   "\<forall> \<sigma> v m. \<sigma> \<in> \<Sigma> \<and> v \<in> V \<and> m \<in> M \<longrightarrow> later_from (m, v, \<sigma>) \<subseteq> M"
+  apply (simp add: later_from_def)
   using later_type from_sender_type by auto
 
 (* Definition 4.6: Latest Messages *)
@@ -50,11 +57,12 @@ definition latest_messages :: "state \<Rightarrow> (validator \<Rightarrow> stat
 
 lemma (in Protocol) latest_messages_type :
   "\<forall> \<sigma> v. \<sigma> \<in> \<Sigma> \<and> v \<in> V \<longrightarrow> latest_messages \<sigma> v \<subseteq> M"
-  using latest_messages_def state_is_subset_of_M by auto
+  apply (simp add: latest_messages_def later_from_def)
+  using from_sender_type by auto
 
-lemma (in Protocol) latest_messages_from_silent_validator_is_empty :
+lemma (in Protocol) latest_messages_from_non_observed_validator_is_empty :
   "\<forall> \<sigma> v. \<sigma> \<in> \<Sigma> \<and> v \<in> V \<and> v \<notin> observed \<sigma> \<longrightarrow> latest_messages \<sigma> v = \<emptyset>"
-  by (simp add: latest_messages_def observed_def)
+  by (simp add: latest_messages_def observed_def later_def from_sender_def)
 
 (* Definition 4.7: Latest message driven estimator *)
 (* TODO *)
@@ -68,38 +76,55 @@ lemma (in Protocol) latest_estimates_type :
   "\<forall> \<sigma> v. \<sigma> \<in> \<Sigma> \<and> v \<in> V \<longrightarrow> latest_estimates \<sigma> v \<subseteq> C"
   using M_type Protocol.latest_messages_type Protocol_axioms latest_estimates_def by fastforce
 
-lemma (in Protocol) latest_estimates_from_silent_validator_is_empty :
+lemma (in Protocol) latest_estimates_from_non_observed_validator_is_empty :
   "\<forall> \<sigma> v. \<sigma> \<in> \<Sigma> \<and> v \<in> V \<and> v \<notin> observed \<sigma> \<longrightarrow> latest_estimates \<sigma> v = \<emptyset>"
-  using latest_estimates_def latest_messages_from_silent_validator_is_empty by auto
+  using latest_estimates_def latest_messages_from_non_observed_validator_is_empty by auto
 
 (* Definition 4.9: Latest estimate driven estimator *)
 (* TODO *)
 
+(* Lemma 10: Observed non-equivocating validators have one latest message *)
+fun observed_non_equivocating_validators :: "state \<Rightarrow> validator set"
+  where
+    "observed_non_equivocating_validators \<sigma> = observed \<sigma> - equivocating_validators \<sigma>"
+
+lemma (in Protocol) observed_non_equivocating_validators_type :
+  "\<forall> \<sigma> \<in> \<Sigma>. observed_non_equivocating_validators \<sigma> \<subseteq> V"
+  using observed_type equivocating_validators_type by auto
+
+
+(* TODO #78: Justification is well-ordered over messages from a non-equivocating validator *)
+lemma (in Protocol) justification_is_well_founded_on_messages_from_non_equivocating_validator:
+  "\<forall> v \<in> V. v \<notin> equivocating_validators \<sigma> \<longrightarrow> wfp_on justified (from_sender (v, \<sigma>))"
+  oops
+
+lemma (in Protocol) justification_is_total_order_on_messages_from_non_equivocating_validator:
+  "\<forall> v \<in> V. v \<notin> equivocating_validators \<sigma> \<longrightarrow> total_on justified (from_sender (v, \<sigma>))"
+  oops
+
+
+(* TODO #59 *)
+lemma (in Protocol) observed_non_equivocating_validators_have_one_latest_message:
+  "\<forall> v \<in> observed_non_equivocating_validators \<sigma>. card (latest_message \<sigma> v) = 1"
+  oops
+
+(* NOTE: Lemma 5 ~ 9 and definition 4.10 are unnecessary so would be omitted. *)
 (* Lemma 5: Non-equivocating validators have at most one latest message *)
 lemma (in Protocol) non_equivocating_validators_have_at_most_one_latest_message:
   "\<forall> v \<in> V. v \<notin> equivocating_validators \<sigma> \<longrightarrow> card (latest_message \<sigma> v) \<le> 1"
   oops
 
-(* Definition 4.10 *)
-(* TODO *)
-
+(* Definition 4.10: The relation \<succeq> (Comparison of cardinalities of justification)*)
 (* Lemma 6 *)
-(* TODO *)
 
 (* Lemma 7 *)
 lemma (in Protocol) monotonicity_of_justifications :
   "\<forall> m m' \<sigma>. m \<in> M \<and> \<sigma> \<in> \<Sigma> \<and> m' \<in> later (m, \<sigma>) \<longrightarrow> justification m \<subseteq> justification m'"
-  apply simp
+  apply (simp add: later_def)
   by (meson M_type justified_def message_in_state_is_valid state_is_in_pow_M_i)
 
 (* Lemma 8 *)
-(* TODO *)
-
 (* Lemma 9 *)
-(* TODO *)
-
-(* Lemma 10 *)
-(* TODO *)
 
 (* Definition 4.11: Latest messages from non-Equivocating validators *)
 definition latest_messages_from_non_equivocating_validators :: "state \<Rightarrow> validator \<Rightarrow> message set"
@@ -122,9 +147,9 @@ lemma (in Protocol) latest_estimates_from_non_equivocating_validators_type :
   "\<forall> \<sigma> v. \<sigma> \<in> \<Sigma> \<and> v \<in> V \<longrightarrow> latest_estimates_from_non_equivocating_validators \<sigma> v \<subseteq> C"
   using Protocol.latest_estimates_type Protocol_axioms latest_estimates_def latest_estimates_from_non_equivocating_validators_def latest_messages_from_non_equivocating_validators_def by auto
 
-lemma (in Protocol) latest_estimates_from_non_equivocating_validators_from_silent_validator_is_empty :
+lemma (in Protocol) latest_estimates_from_non_equivocating_validators_from_non_observed_validator_is_empty :
   "\<forall> \<sigma> v. \<sigma> \<in> \<Sigma> \<and> v \<in> V \<and> v \<notin> observed \<sigma> \<longrightarrow> latest_estimates_from_non_equivocating_validators \<sigma> v = \<emptyset>"
-  by (simp add: latest_estimates_from_non_equivocating_validators_def latest_messages_from_non_equivocating_validators_def latest_messages_from_silent_validator_is_empty)
+  by (simp add: latest_estimates_from_non_equivocating_validators_def latest_messages_from_non_equivocating_validators_def latest_messages_from_non_observed_validator_is_empty)
 
 (* Definition 4.14: Latest honest estimate driven estimator *)
 (* TODO *)
