Isabelle/CBCCasper.thy
@@ -267,7 +267,7 @@ definition observed :: "state \<Rightarrow> validator set"
   where
     "observed \<sigma> = {sender m | m. m \<in> \<sigma>}"
 
-lemma (in Protocol) oberved_type :
+lemma (in Protocol) observed_type :
   "\<forall> \<sigma> \<in> \<Sigma>. observed \<sigma> \<subseteq> V"
   using Params.M_type Protocol_axioms observed_def state_is_subset_of_M by fastforce
 
@@ -291,13 +291,17 @@ definition equivocating_validators :: "state \<Rightarrow> validator set"
   where
     "equivocating_validators \<sigma> = {v \<in> observed \<sigma>. is_equivocating \<sigma> v}"
 
+lemma (in Protocol) equivocating_validators_type :
+  "\<forall> \<sigma> \<in> \<Sigma>. equivocating_validators \<sigma> \<subseteq> V"
+  using observed_type equivocating_validators_def by blast
+
 definition (in Params) equivocating_validators_paper :: "state \<Rightarrow> validator set"
   where
     "equivocating_validators_paper \<sigma> = {v \<in> V. is_equivocating \<sigma> v}"
 
 lemma (in Protocol) equivocating_validators_is_equivalent_to_paper :
   "\<forall> \<sigma> \<in> \<Sigma>. equivocating_validators \<sigma> = equivocating_validators_paper \<sigma>"
-  by (smt Collect_cong Params.equivocating_validators_paper_def equivocating_validators_def is_equivocating_def mem_Collect_eq oberved_type observed_def subsetCE)
+  by (smt Collect_cong Params.equivocating_validators_paper_def equivocating_validators_def is_equivocating_def mem_Collect_eq observed_type observed_def subsetCE)
 
 
 (* Definition 2.11 *)
